Make the definition of correctness to other file & Change the correctness of the function compilation

CompilerProof/CompilerProof.v
@@ -1,53 +1,7 @@
 Require Import Monad DepList GPUCSL TypedTerm Compiler.
 Require Import Program.Equality LibTactics.
-Require Import CUDALib CodeGen CSLLemma CSLTactics.
+Require Import CUDALib CodeGen CSLLemma CSLTactics Correctness.
 Import Skel_lemma.
-
-Notation SVarEnv GS := (hlist (fun typ : Skel.Typ => vars typ) GS).
-Notation SEvalEnv GS := (hlist Skel.typDenote GS).
-Notation AVarEnv GA := (hlist (fun typ : Skel.Typ => (var * vars typ)%type) GA).
-Notation APtrEnv GA := (hlist (fun typ => vals typ) GA).
-Notation AEvalEnv GA := (hlist Skel.aTypDenote GA).
-
-Fixpoint fold_hlist {A B C} (ls : list A) (g : B -> C -> C) (d : C) :=
-  match ls return (forall x, member x ls -> B) -> C with
-  | nil => fun _ => d
-  | x :: ls => fun f => g (f x HFirst) (fold_hlist ls g d (fun x m => f x (HNext m)))
-  end.
-
-(* Bad naming: convert TypedIR level value to CUDA level value
- *)
-Fixpoint sc2CUDA {ty} :=
-  match ty return Skel.typDenote ty -> vals ty with
-  | Skel.TBool => fun b => if b then 1 else 0
-  | Skel.TZ => fun n => n
-  | Skel.TTup t1 t2 => fun p => (sc2CUDA (fst p), sc2CUDA (snd p))
-  end%Z.
-
-Definition arr2CUDA {ty} : Skel.aTypDenote ty -> list (vals ty) := map sc2CUDA.
-
-Definition val2sh {ty} := @maptys ty _ _ SLoc.
-Definition val2gl {ty} := @maptys ty _ _ GLoc.
-
-Definition arrInvRes {GA} (aPtrEnv : APtrEnv GA) (aEvalEnv : AEvalEnv GA) : res :=
-  fold_hlist GA Star Emp
-    (fun x m => arrays (val2gl (hget aPtrEnv m)) (arr2CUDA (hget aEvalEnv m)) 1).
-
-Definition arrInvVar {GA} (aVarEnv : AVarEnv GA) (aPtrEnv : APtrEnv GA) (aEvalEnv : AEvalEnv GA) : list entry :=
-  fold_hlist GA (@app entry) nil
-    (fun x m => let (xlen, xarr) := hget aVarEnv m in
-                xlen |-> Zn (length (hget aEvalEnv m)) :: xarr |=> hget aPtrEnv m).
-
-Definition scInv {GS} (sVarEnv : SVarEnv GS) (sEvalEnv : SEvalEnv GS) :=
-  fold_hlist GS (@app entry) nil
-    (fun x m => (hget sVarEnv m) |=> sc2CUDA (hget sEvalEnv m)). 
-
-Definition kernelInv {GS GA}
-           (sVarEnv : SVarEnv GS) (sEvalEnv : SEvalEnv GS)
-           (aVarEnv : AVarEnv GA) (aPtrEnv : APtrEnv GA) (aEvalEnv : AEvalEnv GA) P resEnv :=
-  Assn (arrInvRes aPtrEnv aEvalEnv)
-       P
-       (resEnv ++ scInv sVarEnv sEvalEnv ++ arrInvVar aVarEnv aPtrEnv aEvalEnv).
 
 Variable sorry : forall A, A.
 Arguments sorry {A}.
@@ -460,16 +414,6 @@ Ltac simplify :=
         | [|- ~_] => intros ?
         end; simpl in *; try substs).
 
-Definition aenv_ok {GA} (avar_env : AVarEnv GA) :=
-  (forall ty (m : member ty GA), prefix "l" (str_of_var (fst (hget avar_env m))) = false)
-  /\ (forall (ty : Skel.Typ) (m : member ty GA) (y : var),
-         In y (flatTup (snd (hget avar_env m)))
-         -> prefix "l" (str_of_var y) = false).
-
-Definition senv_ok {GS} (svar_env : SVarEnv GS) n :=
-  (forall (ty : Skel.Typ) (m : member ty GS) (k : nat) l,
-      In (Var (lpref k ++ l)) (flatTup (hget svar_env m)) -> k < n).
-
 Lemma compile_gens GA GS typ (se : Skel.SExp GA GS typ) avar_env svar_env n0 n1 c es :
   compile_sexp se avar_env svar_env n0 = ((c, es), n1) ->
   senv_ok svar_env n0 -> (* fvs are not in the future generated vars *)
@@ -743,10 +687,6 @@ Proof.
   (try now (destruct (Z_lt_dec _ _), (Z.ltb_spec v1 v2); substs; try tauto; omega)).
 Qed.
 
-Definition resEnv_ok resEnv n := 
-  forall v (k : nat) l,
-    In ((lpref k ++ l)%string |-> v) resEnv -> k < n.
-
 Lemma remove_gen_vars_res resEnv ty n m xs :
   freshes ty n = (xs, m) ->
   resEnv_ok resEnv n ->
@@ -807,7 +747,6 @@ Proof.
   rewrite in_app_iff in *.
   destruct H; [forwards*: He| forwards*: Hres].
 Qed.    
-
     
 Lemma compile_gen_resEnv_ok GA GS (avar_env : AVarEnv GA) (svar_env : SVarEnv GS)
       ty (se : Skel.SExp GA GS ty) c (xs : vars ty) v n m k :
@@ -1091,14 +1030,14 @@ Lemma compile_sexp_ok ntrd BS (tid : Fin.t ntrd) GA GS typ (se : Skel.SExp GA GS
   resEnv_ok resEnv n ->
   (* (iii) return exps. don't have future generated vars*)
   CSL BS tid  (* correctness of gen. code *)
-      (kernelInv svar_env seval_env avar_env aptr_env aeval_env P resEnv)
+      (sexpInv svar_env seval_env avar_env aptr_env aeval_env P resEnv)
       c
-      (kernelInv svar_env seval_env avar_env aptr_env aeval_env P (es |=> sc2CUDA v ++ resEnv)).
+      (sexpInv svar_env seval_env avar_env aptr_env aeval_env P (es |=> sc2CUDA v ++ resEnv)).
 Proof.
   revert typ se seval_env svar_env n m v c es P resEnv.
   induction se;
   introv Heval Hcompile Hsok Haok Hresok;
-  unfold bind_opt in Hcompile; unfold kernelInv in *; unfoldM_in Hcompile.
+  unfold bind_opt in Hcompile; unfold sexpInv in *; unfoldM_in Hcompile.
   - (* case of var *)
     inverts Hcompile.
     inverts Heval.
@@ -1305,55 +1244,6 @@ Proof.
     unfold scInv in *; simpl in *; rewrite in_app_iff in *; tauto.
 Qed.
 
-Definition is_local (x : var) : Prop := prefix "l" (str_of_var x) = true.
-Definition are_local {ty} (xs : vars ty) : Prop :=
-  forall x, In x (flatTup xs) -> is_local x.
-
-Definition func_ok1 {GA dom cod} (avar_env : AVarEnv GA) 
-           (f : Skel.Func GA (Skel.Fun1 dom cod)) (func : type_of_ftyp (Skel.Fun1 dom cod)) :=
-  aenv_ok avar_env 
-  -> (* func only writes to local variables *)
-     (forall x l, In l (writes_var (fst (func x))) -> is_local l) /\
-     (* func only returs to local variables or parameter *)
-     (forall x l, In l (flatTup (snd (func x))) -> is_local l) /\
-     (* functional correctenss *)
-     (forall ntrd (tid : Fin.t ntrd) BS xs vs res aptr_env aeval_env P resEnv,
-         (forall l, In l (flatTup xs) -> ~is_local l)
-         -> resEnv_ok resEnv 0
-         -> (Skel.funcDenote _ _ f aeval_env vs = Some res)
-         -> CSL BS tid
-                (kernelInv (xs ::: HNil) (vs ::: HNil) avar_env aptr_env aeval_env P resEnv)
-                (fst (func xs))
-                (kernelInv (xs ::: HNil) (vs ::: HNil) avar_env aptr_env aeval_env P
-                           (snd (func xs) |=> sc2CUDA res ++ resEnv))) /\
-     (forall x, barriers (fst (func x)) = nil).
-
-Definition func_ok2 {GA dom1 dom2 cod} (avar_env : AVarEnv GA) 
-           (f : Skel.Func GA (Skel.Fun2 dom1 dom2 cod)) (func : type_of_ftyp (Skel.Fun2 dom1 dom2 cod)) :=
-  aenv_ok avar_env 
-  -> (* func only writes to local variables *)
-     (forall x y l, In l (writes_var (fst (func x y))) -> is_local l) /\
-     (* func only returs to local variables or parameter *)
-     (forall x y l, In l (flatTup (snd (func x y))) -> is_local l) /\
-     (* functional correctenss *)
-     (forall ntrd (tid : Fin.t ntrd) BS xs ys vs1 vs2 res aptr_env aeval_env P resEnv,
-         (forall l, In l (flatTup xs) -> ~is_local l)
-         -> (forall l, In l (flatTup ys) -> ~is_local l)
-         -> resEnv_ok resEnv 0
-         -> (Skel.funcDenote _ _ f aeval_env vs1 vs2 = Some res)
-         -> CSL BS tid
-                (kernelInv (ys ::: xs ::: HNil) (vs2 ::: vs1 ::: HNil) avar_env aptr_env aeval_env P resEnv)
-                (fst (func xs ys))
-                (kernelInv (ys ::: xs ::: HNil) (vs2 ::: vs1 ::: HNil) avar_env aptr_env aeval_env P
-                           (snd (func xs ys) |=> sc2CUDA res ++ resEnv))) /\
-     (forall xs ys, barriers (fst (func xs ys)) = nil).
-
-Definition func_ok {GA fty} (avar_env : AVarEnv GA) :=
-  match fty return Skel.Func GA fty -> type_of_ftyp fty -> Prop with
-  | Skel.Fun1 dom cod => fun f func => func_ok1 avar_env f func
-  | Skel.Fun2 dom1 dom2 cod => fun f func => func_ok2 avar_env f func 
-  end.
-
 Lemma freshes_prefix ty n m res :
   freshes ty n = (res, m) 
   -> forall l, In l (flatTup res) -> is_local l.
@@ -1483,10 +1373,11 @@ Proof.
   destruct (compile_sexp _ _ _ _) as [[? ?] ?] eqn:Heq; simpl in *;
   eauto using compile_sexp_no_barrs, compile_sexp_wr_vars, compile_sexp_res_vars, compile_sexp_ok;
   unfold are_local; [intros Hx ? ?| intros Hx Hy ? ?];
-  forwards*: compile_sexp_ok;
-  unfold senv_ok, is_local in *; introv Hin; false;
-  repeat des_mem; simpl in *;
-  try no_side_cond ltac:(forwards* Hin': Hx);
-  try no_side_cond ltac:(forwards* Hin': Hy);
-  unfold lpref in Hin'; simpl in *; rewrite prefix_nil in Hin'; congruence.
+  forwards*Htri: compile_sexp_ok; unfold kernelInv, sexpInv, scInv in *; simpl in *;
+  first [eapply rule_conseq; try apply Htri; prove_imp; simpl in *; try tauto | (* discharging triples *)
+         unfold senv_ok, is_local in *; introv Hin; false;
+         repeat des_mem; simpl in *;
+         try no_side_cond ltac:(forwards* Hin': Hx);
+         try no_side_cond ltac:(forwards* Hin': Hy);
+         unfold lpref in Hin'; simpl in *; rewrite prefix_nil in Hin'; congruence].
 Qed.
