CompilerProof/Correctness.v
@@ -1,0 +1,122 @@
+Require Import Monad DepList GPUCSL TypedTerm Compiler.
+Require Import Program.Equality LibTactics.
+Require Import CUDALib CodeGen CSLLemma CSLTactics.
+Import Skel_lemma.
+
+Notation SVarEnv GS := (hlist (fun typ : Skel.Typ => vars typ) GS).
+Notation SEvalEnv GS := (hlist Skel.typDenote GS).
+Notation AVarEnv GA := (hlist (fun typ : Skel.Typ => (var * vars typ)%type) GA).
+Notation APtrEnv GA := (hlist (fun typ => vals typ) GA).
+Notation AEvalEnv GA := (hlist Skel.aTypDenote GA).
+
+Fixpoint fold_hlist {A B C} (ls : list A) (g : B -> C -> C) (d : C) :=
+  match ls return (forall x, member x ls -> B) -> C with
+  | nil => fun _ => d
+  | x :: ls => fun f => g (f x HFirst) (fold_hlist ls g d (fun x m => f x (HNext m)))
+  end.
+
+(* Bad naming: convert TypedIR level value to CUDA level value
+ *)
+Fixpoint sc2CUDA {ty} :=
+  match ty return Skel.typDenote ty -> vals ty with
+  | Skel.TBool => fun b => if b then 1 else 0
+  | Skel.TZ => fun n => n
+  | Skel.TTup t1 t2 => fun p => (sc2CUDA (fst p), sc2CUDA (snd p))
+  end%Z.
+
+Definition arr2CUDA {ty} : Skel.aTypDenote ty -> list (vals ty) := map sc2CUDA.
+
+Definition val2sh {ty} := @maptys ty _ _ SLoc.
+Definition val2gl {ty} := @maptys ty _ _ GLoc.
+
+Definition arrInvRes {GA} (aPtrEnv : APtrEnv GA) (aEvalEnv : AEvalEnv GA) : res :=
+  fold_hlist GA Star Emp
+    (fun x m => arrays (val2gl (hget aPtrEnv m)) (arr2CUDA (hget aEvalEnv m)) 1).
+
+Definition arrInvVar {GA} (aVarEnv : AVarEnv GA) (aPtrEnv : APtrEnv GA) (aEvalEnv : AEvalEnv GA) : list entry :=
+  fold_hlist GA (@app entry) nil
+    (fun x m => let (xlen, xarr) := hget aVarEnv m in
+                xlen |-> Zn (length (hget aEvalEnv m)) :: xarr |=> hget aPtrEnv m).
+
+Definition scInv {GS} (sVarEnv : SVarEnv GS) (sEvalEnv : SEvalEnv GS) :=
+  fold_hlist GS (@app entry) nil
+    (fun x m => (hget sVarEnv m) |=> sc2CUDA (hget sEvalEnv m)). 
+
+Definition sexpInv {GS GA}
+           (sVarEnv : SVarEnv GS) (sEvalEnv : SEvalEnv GS)
+           (aVarEnv : AVarEnv GA) (aPtrEnv : APtrEnv GA) (aEvalEnv : AEvalEnv GA) P resEnv :=
+  Assn (arrInvRes aPtrEnv aEvalEnv)
+       P
+       (resEnv ++ scInv sVarEnv sEvalEnv ++ arrInvVar aVarEnv aPtrEnv aEvalEnv).
+
+Definition kernelInv {GA} 
+           (aVarEnv : AVarEnv GA) (aPtrEnv : APtrEnv GA) (aEvalEnv : AEvalEnv GA) P resEnv := 
+  Assn (arrInvRes aPtrEnv aEvalEnv) P (resEnv ++ arrInvVar aVarEnv aPtrEnv aEvalEnv).
+
+Definition aenv_ok {GA} (avar_env : AVarEnv GA) :=
+  (forall ty (m : member ty GA), prefix "l" (str_of_var (fst (hget avar_env m))) = false)
+  /\ (forall (ty : Skel.Typ) (m : member ty GA) (y : var),
+         In y (flatTup (snd (hget avar_env m)))
+         -> prefix "l" (str_of_var y) = false).
+
+Definition senv_ok {GS} (svar_env : SVarEnv GS) n :=
+  (forall (ty : Skel.Typ) (m : member ty GS) (k : nat) l,
+      In (Var (lpref k ++ l)) (flatTup (hget svar_env m)) -> k < n).
+
+Definition resEnv_ok resEnv n := 
+  forall v (k : nat) l,
+    In ((lpref k ++ l)%string |-> v) resEnv -> k < n.
+
+
+Definition is_local (x : var) : Prop := prefix "l" (str_of_var x) = true.
+Definition are_local {ty} (xs : vars ty) : Prop :=
+  forall x, In x (flatTup xs) -> is_local x.
+
+Definition func_ok1 {GA dom cod} (avar_env : AVarEnv GA) 
+           (f : Skel.Func GA (Skel.Fun1 dom cod)) (func : type_of_ftyp (Skel.Fun1 dom cod)) :=
+  aenv_ok avar_env 
+  -> (* func only writes to local variables *)
+     (forall x l, In l (writes_var (fst (func x))) -> is_local l) /\
+     (* func only returs to local variables or parameter *)
+     (forall x l, In l (flatTup (snd (func x))) -> is_local l) /\
+     (* functional correctenss *)
+     (forall ntrd (tid : Fin.t ntrd) BS xs vs res aptr_env aeval_env P resEnv,
+         (forall l, In l (flatTup xs) -> ~is_local l)
+         -> resEnv_ok resEnv 0
+         -> (Skel.funcDenote _ _ f aeval_env vs = Some res)
+         -> CSL BS tid
+                (kernelInv avar_env aptr_env aeval_env P 
+                           (xs |=> sc2CUDA vs ++ resEnv))
+                (fst (func xs))
+                (kernelInv avar_env aptr_env aeval_env P
+                           (snd (func xs) |=> sc2CUDA res ++
+                            xs |=> sc2CUDA vs ++ resEnv))) /\
+     (forall x, barriers (fst (func x)) = nil).
+
+Definition func_ok2 {GA dom1 dom2 cod} (avar_env : AVarEnv GA) 
+           (f : Skel.Func GA (Skel.Fun2 dom1 dom2 cod)) (func : type_of_ftyp (Skel.Fun2 dom1 dom2 cod)) :=
+  aenv_ok avar_env 
+  -> (* func only writes to local variables *)
+     (forall x y l, In l (writes_var (fst (func x y))) -> is_local l) /\
+     (* func only returs to local variables or parameter *)
+     (forall x y l, In l (flatTup (snd (func x y))) -> is_local l) /\
+     (* functional correctenss *)
+     (forall ntrd (tid : Fin.t ntrd) BS xs ys vs1 vs2 res aptr_env aeval_env P resEnv,
+         (forall l, In l (flatTup xs) -> ~is_local l)
+         -> (forall l, In l (flatTup ys) -> ~is_local l)
+         -> resEnv_ok resEnv 0
+         -> (Skel.funcDenote _ _ f aeval_env vs1 vs2 = Some res)
+         -> CSL BS tid
+                (kernelInv avar_env aptr_env aeval_env P 
+                           (xs |=> sc2CUDA vs1 ++ ys |=> sc2CUDA vs2 ++ resEnv))
+                (fst (func xs ys))
+                (kernelInv avar_env aptr_env aeval_env P
+                           (snd (func xs ys) |=> sc2CUDA res ++ 
+                            xs |=> sc2CUDA vs1 ++ ys |=> sc2CUDA vs2 ++ resEnv))) /\
+     (forall xs ys, barriers (fst (func xs ys)) = nil).
+
+Definition func_ok {GA fty} (avar_env : AVarEnv GA) :=
+  match fty return Skel.Func GA fty -> type_of_ftyp fty -> Prop with
+  | Skel.Fun1 dom cod => fun f func => func_ok1 avar_env f func
+  | Skel.Fun2 dom1 dom2 cod => fun f func => func_ok2 avar_env f func 
+  end.
